\documentclass{article}
\usepackage{amsmath}
\usepackage{graphicx} % Required for inserting images

\title{ATE}
\author{7557756}
\date{July 2024}

\begin{document}

\maketitle

\section{Formulas}

\begin{align*}
p = \text{the proportion treated (i.e., the proportion of cases } D=1), \\
q = \text{the proportion untreated (i.e., the proportion of cases } D=0), \\
\end{align*}
\begin{align*}
E(Y^1_{D=1}) = E(Y^1 \mid D=1), \\
E(Y^0_{D=1}) = E(Y^0 \mid D=1), \\
E(Y^1_{D=0}) = E(Y^1 \mid D=0), \\
E(Y^0_{D=0}) = E(Y^0 \mid D=0).
\end{align*}

\begin{align*}
E(Y^1_{D=1})p = E(Y^1_{D=1}) - E(Y^1_{D=1})q 
\end{align*}

\begin{align*}
HTE = -E(Y^1_{D=1})q + E(Y^0_{D=1})q + E(Y^1_{D=0})q - E(Y^0_{D=0})q \\
= -q[+E(Y^1_{D=1}) - E(Y^0_{D=1}) - E(Y^1_{D=0}) + E(Y^0_{D=0})] \\
= -q[(E(Y^1_{D=1}) - E(Y^0_{D=1})) - ( E(Y^1_{D=0}) - E(Y^0_{D=0}))] 
\end{align*}

\begin{align*}
= E(Y^1_{D=1}) - E(Y^0_{D=1})
\end{align*}

\begin{align*}
E(Y^0_{D=1}) =  E(Y^0_{D=0}) + (E(Y^0_{D=1})- E(Y^0_{D=0}))
\end{align*}

\begin{align*}
= E(Y^1_{D=1}) - E(Y^0_{D=0}) - (E(Y^0_{D=1})- E(Y^0_{D=0}))
\end{align*}
    
\end{document}
